mcontests.v
@@ -1,0 +1,64 @@
+Load mconbase.
+
+(*Check E_ident(0).*)
+Check JO_red (E_ident(0)) (E_ident(1)).
+
+
+Theorem identisexpr : forall (n : nat), is_expr_of_expr (E_ident(n)) = True.
+Proof.
+ intros n.
+ simpl.
+ trivial.
+Qed.
+
+Extraction Language Ocaml.
+
+Notation "A >>= F" := (E_bind A F) (at level 42, left associativity).
+
+Example valuepair : is_value_of_expr (E_pair (E_constant(CONST_ret)) (E_constant(CONST_fork))).
+Proof.
+ simpl.
+ auto.
+Qed.
+
+Ltac caseEq f :=
+  generalize (refl_equal f); pattern f at -1; case f. 
+
+Inductive JO_red_star : expr -> expr -> Prop :=
+| JO_red_star_step: forall e e' f,
+    JO_red e e' ->
+    JO_red_star e' f ->
+    JO_red_star e f
+| JO_red_star_refl: forall e,
+    JO_red_star e e.
+
+Example simplred : forall (x:value_name) (e v:expr),
+     is_value_of_expr v ->
+     JO_red (E_apply  (E_function x e)  v)  (subst_expr  v   x   e ).
+Proof.
+  intros.
+  Check JO_red_app.
+  apply JO_red_app.
+  apply H.
+Qed.
+
+Lemma mon_left_id : forall (x:value_name) (a e:expr),
+    is_value_of_expr a ->
+    JO_red_star ((E_apply(E_constant (CONST_ret)) a) >>= (E_function x e)) (E_apply (E_function x e) a).
+Proof.
+ intros.
+ apply JO_red_star_step with (e' := (E_bind (E_live_expr a) (E_function x e))).
+ apply JO_red_evalbind.
+ apply JO_red_ret.
+ apply H.
+ apply JO_red_star_step with (e' := (E_apply (E_function x e) a)).
+ apply JO_red_dobind.
+ apply H.
+ apply JO_red_star_refl.
+Qed.
+
+(*
+Lemma mon_right_id : forall (a:expr),
+   is_value_of_expr a ->
+   JO_red_star (E_bind (a)  (E_constant (CONST_ret))) (a).
+*)
